rebuilt against new HOL and cakeML, cleanup

HOL/panScript.sml
@@ -5,8 +5,9 @@
 open panItreeSemTheory;
 open panSemTheory; (* eval_def *)
 
-(*/ equational
-   not sure whether this should be kept around but lemmas use it atm
+(*/ equational theorems for mrec
+   mrec expresses a recursive computation by iterating Vis INL
+   TODO should this be in the itreeTauTheory? Yes
  *)
 
 (* iiter (Ret INL) → Tau (itree_unfold (iiter_cb (mrec_cb h_prog))
@@ -27,29 +28,16 @@ Proof
   AP_THM_TAC >>
   AP_TERM_TAC >>
   rw[FUN_EQ_THM] >>
-  rw[DefnBase.one_line_ify NONE mrec_cb_def]
+  rw[DefnBase.one_line_ify NONE mrec_cb_def, combinTheory.o_DEF]
 QED
 
 Theorem iter_mrec_cb_thm[simp]:
-  iter (mrec_cb h_prog) (Ret x) = Ret x ∧
-  iter (mrec_cb h_prog) (Tau t) = Tau (iter (mrec_cb h_prog) t) ∧
-  iter (mrec_cb h_prog) (Vis (INL s) g)
-    = Tau (iter (mrec_cb h_prog) (bind (h_prog s) g)) ∧
-  iter (mrec_cb h_prog) (Vis (INR e) k)
-    = Vis e (λx. Tau (iter (mrec_cb h_prog) (k x)))
+  iter (mrec_cb rh) (Ret x) = Ret x ∧
+  iter (mrec_cb rh) (Tau t) = Tau (iter (mrec_cb rh) t) ∧
+  iter (mrec_cb rh) (Vis (INL s) g) = Tau (iter (mrec_cb rh) (bind (rh s) g)) ∧
+  iter (mrec_cb rh) (Vis (INR e) k) = Vis e (λx. Tau (iter (mrec_cb rh) (k x)))
 Proof
   rw[Once itree_iter_thm] >> rw[Once itree_iter_thm]
-QED
-
-(*/ Seq thm
-   this is how we split up a program
- *)
-
-(* inversion lemmas *)
-Theorem itree_bind_ret_inv:
-  bind t k = Ret r ⇒ ∃r'. t = Ret r' ∧ Ret r = (k r')
-Proof
-  Cases_on ‘t’ >> fs[]
 QED
 
 Theorem mrec_cb_ret_inv:
@@ -60,19 +48,19 @@ Proof
    (Cases_on ‘a’ >> fs[])
 QED
 
-(* h_prog iterates sequentially on its seed *)
-Theorem mrec_bind_thm:
-  ∀t k. iter (mrec_cb h_prog) (bind t k) =
-        bind (iter (mrec_cb h_prog) t) (λx. iter (mrec_cb h_prog) (k x))
+(* mrec iterates sequentially on its seed *)
+Theorem itree_mrec_bind:
+  iter (mrec_cb rh) (bind t k) =
+  bind (iter (mrec_cb rh) t) (λx. iter (mrec_cb rh) (k x))
 Proof
   rw[Once itree_strong_bisimulation] >>
-  qexists_tac ‘λa b. ∃ps. a = iter (mrec_cb h_prog) (bind ps k) ∧
-                          b = bind (iter (mrec_cb h_prog) ps)
-                                (λx. iter (mrec_cb h_prog) (k x))’ >>
+  qexists_tac ‘λa b. ∃ps. a = iter (mrec_cb rh) (bind ps k) ∧
+                          b = bind (iter (mrec_cb rh) ps)
+                                (λx. iter (mrec_cb rh) (k x))’ >>
   rw[] >-
    (metis_tac[]) >-
-   (‘bind (mrec_cb h_prog (bind ps k))
-       (λx. case x of INL a => Tau (iter (mrec_cb h_prog) a) | INR b => Ret b)
+   (‘bind (mrec_cb rh (bind ps k))
+       (λx. case x of INL a => Tau (iter (mrec_cb rh) a) | INR b => Ret b)
      = Ret x’
       by gvs[Once itree_iter_thm] >>
     qpat_x_assum ‘Ret x = iter _ _’ kall_tac >>
@@ -95,35 +83,25 @@ Proof
       rw[]))
 QED
 
-Theorem mrec_seq_thm:
-  iter (mrec_cb h_prog)
-     (bind t
-        (λ(res,s'). if res = NONE then Vis (INL (p2,s')) Ret else Ret (res,s')))
-  = bind (iter (mrec_cb h_prog) t)
-      (λ(res,s').
-         if res = NONE then Tau (iter (mrec_cb h_prog) (h_prog (p2,s')))
-         else Ret (res,s'))
-Proof
-  rw[mrec_bind_thm] >>
-  AP_TERM_TAC >>
-  rw[FUN_EQ_THM] >>
-  Cases_on ‘x’ >> rw[]
-QED
+(*/ pancake theorems
+   equational pancake itrees
+ *)
 
 Theorem seq_thm:
   itree_mrec h_prog (Seq p p2, s) =
   Tau (bind (itree_mrec h_prog (p, s))
-         (λ(res,s').
-            if res = NONE
-            then Tau (itree_mrec h_prog (p2, s'))
-            else (Ret (res, s'))))
+            (λ(res,s').
+               if res = NONE
+               then Tau (itree_mrec h_prog (p2, s'))
+               else (Ret (res, s'))))
 Proof
   rw[itree_mrec_alt] >>
   rw[h_prog_def, h_prog_rule_seq_def] >>
-  rw[mrec_seq_thm]
+  rw[itree_mrec_bind] >>
+  AP_TERM_TAC >>
+  rw[FUN_EQ_THM] >>
+  Cases_on ‘x’ >> rw[]
 QED
-
-(* Dec cleanup *)
 
 Definition revert_binding_def:
   revert_binding name old_s
@@ -147,13 +125,13 @@ QED
 
 (* f, f' type vars instantiated differently smh *)
 (* relies on mrec_cb h_prog rev -> only Ret INR, so can't prolong iteration *)
-Theorem mrec_bind_ret:
+Theorem itree_mrec_bind_ret:
   ∀f f'.
     (∀a. ∃r. (f a) = (Ret r) ∧ (f' a) = (Ret r)) ⇒
     ∀t. iter (mrec_cb h_prog) (bind t f) = (bind (iter (mrec_cb h_prog) t) f')
 Proof
   rpt strip_tac >>
-  rw[mrec_bind_thm] >>
+  rw[itree_mrec_bind] >>
   AP_TERM_TAC >> rw[FUN_EQ_THM] >>
   pop_assum $ qspec_then ‘x’ strip_assume_tac >> fs[]
 QED
@@ -168,29 +146,36 @@ Proof
   rw[itree_mrec_alt] >>
   rw[h_prog_def, h_prog_rule_dec_def] >>
   rw[GSYM revert_binding_def] >>
-  irule mrec_bind_ret >>
+  irule itree_mrec_bind_ret >>
   rw[revert_binding_def] >>
   Cases_on ‘a’ >> rw[]
 QED
 
 (*/ massaging into ffi itree
-   TODO change when fixed
+   TODO merge
  *)
 
 Definition massage_cb_def[simp]:
-    massage_cb (INL stree) = massage stree ∧
-    massage_cb (INR (Ret res_state,st)) = massage (st res_state) ∧
-    massage_cb (INR (Tau kt,st)) = Tau' (INR (kt,st)) ∧
-    massage_cb (INR (Vis svis_ev kt',st))
-    = Vis' svis_ev (λffi_res. INR (kt' ffi_res,st))
+  massage_cb (Ret (res, s)) = Ret' res ∧
+  massage_cb (Tau kt) = Tau' kt ∧
+  massage_cb (Vis (svis_ev, scb) st) = Vis' svis_ev (λffi_res. st (scb ffi_res))
 End
 
 (* massage Ret type from (η x state) -> η *)
 (* convert Vis (sem_vis_event x (FFI_result -> itree)) ((prog x state) -> %itree)
 -> Vis sem_vis_event (FFI_result -> itree) *)
 Definition to_ffi_def:
-  to_ffi x = itree_unfold massage_cb (INL x)
+  to_ffi t = itree_unfold massage_cb t
 End
+
+Theorem to_ffi_alt[simp]:
+  to_ffi (Tau t) = Tau (to_ffi t) ∧
+  to_ffi (Ret (p,s)) = Ret p ∧
+  to_ffi (Vis (svis_ev,scb) g) = Vis svis_ev (λffi_res. to_ffi (g (scb (ffi_res))))
+Proof
+  rw[to_ffi_def] >> rw[Once itree_unfold] >>
+  rw[combinTheory.o_DEF]
+QED
 
 Theorem itree_evaluate_alt:
   itree_evaluate p s = to_ffi (itree_mrec h_prog (p,s))
@@ -199,7 +184,7 @@ Proof
   AP_THM_TAC >> (* same fn => same on same arg, backwards *)
   AP_TERM_TAC >>
   rw[FUN_EQ_THM] >>
-  rw[DefnBase.one_line_ify NONE massage_cb_def]
+  rw[DefnBase.one_line_ify NONE massage_cb_def, combinTheory.o_DEF]
 QED
 
 open finite_mapTheory; (* FLOOKUP_UPDATE *)
@@ -229,119 +214,16 @@ fun parse_pancake q =
     EVAL “parse_funs_to_ast ^code”
 end
 
-(*/ loops work!
-   manual loop unrolling isn't too bad with equational rewrites
+(*/
+  ffi skip test
  *)
-
-val loop_ast = rhs $ concl $ parse_pancake ‘
-fun fn() {
-  var x = 1;
-  x = 0;
-  while (x < 1) {
-    x = x + 1;
-  }
-}’;
-
-Definition loop_sem_def:
-  loop_sem (s:('a,'ffi) panSem$state) =
-  itree_evaluate (SND $ SND $ HD $ THE ^loop_ast) s
-End
-
-Definition h_prog_whilebody_cb_def[simp]:
-    h_prog_whilebody_cb p (SOME Break) s' = Ret (INR (NONE,s'))
-  ∧ h_prog_whilebody_cb p (SOME Continue) s' = Ret (INL (p,s'))
-  ∧ h_prog_whilebody_cb p NONE s' = Ret (INL (p,s'))
-  (* nice! this syntax is valid *)
-  ∧ h_prog_whilebody_cb p res s' = Ret (INR (res,s'))
-End
-
-Definition h_prog_while_cb_def[simp]:
-    h_prog_while_cb (p,s) NONE = Ret (INR (SOME Error,s))
-  ∧ h_prog_while_cb (p,s) (SOME (ValWord w))
-    = (if (w ≠ 0w)
-       then Vis (INL (p,s))
-                (λ(res,s'). h_prog_whilebody_cb p res s')
-       else Ret (INR (NONE,s)))
-  ∧ h_prog_while_cb (p,s) (SOME (ValLabel _)) = Ret (INR (SOME Error,s))
-  ∧ h_prog_while_cb (p,s) (SOME (Struct _)) = Ret (INR (SOME Error,s))
-End
-
-(* PR submitted *)
-Theorem h_prog_rule_while_alt:
-  h_prog_rule_while g p s =
-  iter (λ(p',s'). (h_prog_while_cb (p',s') (eval s' g))) (p,s)
-Proof
-  rw[h_prog_rule_while_def] >>
-  AP_THM_TAC >>
-  AP_TERM_TAC >>
-  rw[FUN_EQ_THM] >>
-  rw[DefnBase.one_line_ify NONE h_prog_while_cb_def] >>
-  rw[DefnBase.one_line_ify NONE h_prog_whilebody_cb_def] >>
-  rpt (PURE_TOP_CASE_TAC >> gvs[] >> rw[FUN_EQ_THM])
-QED
-
-Theorem cheat1:
-  0w < 1w (* supposed to be :4 word but weever *)
-Proof
-  cheat
-QED
-
-Theorem mrec_thm:
-  iter (mrec_cb h_prog) (bind t k)
-  ≈ bind (iter (mrec_cb h_prog) t) (λr. iter (mrec_cb h_prog) (k r))
-Proof
-  CONV_TAC $ RHS_CONV $ REWRITE_CONV[Once itree_iter_thm, mrec_cb_def] >>
-  CONV_TAC $ RHS_CONV $ REWRITE_CONV[Once itree_bind_thm] >>
-  rw[itree_bind_thm]
-QED
-
-Theorem loop_thm:
-  loop_sem s =  Tau (Tau (Tau (Tau (Tau (Ret NONE)))))
-Proof
-  rw[loop_sem_def, itree_semantics_def, itree_evaluate_alt] >>
-  rw[itree_mrec_alt, h_prog_def, h_prog_rule_dec_alt] >>
-  rw[eval_def] >>
-  rw[Once itree_iter_thm, itree_bind_thm] >>
-  (* seq *)
-  rw[h_prog_def, h_prog_rule_seq_def] >>
-  rw[itree_bind_thm] >>
-  rw[Once itree_iter_thm] >>
-  rw[Once itree_bind_thm] >>
-  (* assign *)
-  rw[Once h_prog_def, h_prog_rule_assign_def] >>
-  rw[FLOOKUP_UPDATE, word_op_def, is_valid_value_def, shape_of_def,
-     Once eval_def, cheat1] >>
-  rw[itree_bind_thm] >>
-  rw[Once itree_iter_thm, Once itree_bind_thm] >>
-  (* while *)
-  rw[Once h_prog_def, h_prog_rule_while_alt] >>
-  rw[Once itree_iter_thm] >> rw[Once itree_iter_thm] >>
-  rw[Once eval_def] >> rw[Once eval_def] >>
-  rw[FLOOKUP_UPDATE] >>
-  rw[Once eval_def, word_cmp_def, cheat1] >>
-  rw[itree_bind_thm] >>
-  (* assignment *)
-  rw[Once h_prog_def, h_prog_rule_assign_def] >>
-  rw[Once eval_def] >> rw[Once eval_def] >>
-  rw[FLOOKUP_UPDATE, word_op_def, is_valid_value_def, shape_of_def,
-     Once eval_def, cheat1] >>
-  rw[Once itree_iter_thm, itree_bind_thm] >>
-  (* second while *)
-  (* rw[GSYM h_prog_rule_while_alt, GSYM h_prog_def] *)
-  rw[Once itree_iter_thm] >> rw[Once itree_iter_thm] >>
-  rw[eval_def, FLOOKUP_UPDATE, word_cmp_def] >>
-  rw[revert_binding_def] >>
-  rw[Once itree_iter_thm, itree_bind_thm] >>
-  (* massage *)
-  rw[massage_thm]
-QED
-
-(* ffi test *)
 
 val ffi_ast = rhs $ concl $ parse_pancake ‘
 fun fn() {
-  #num_clients(0, 0, 0, 0);
-  #num_clients(0, 0, 0, 0);
+  #f1(0, 0, 0, 0);
+  #f2(0, 0, 0, 0);
+  #f3(0, 0, 0, 0);
+  #f4(0, 0, 0, 0);
 }’;
 
 Definition ffi_sem_def:
@@ -349,10 +231,80 @@ Definition ffi_sem_def:
   itree_evaluate (SND $ SND $ HD $ THE ^ffi_ast) s
 End
 
-Theorem ffi_sem_thm:
-  ffi_sem s = ARB
+(* Inductive walk: *)
+(* [~Tau:] (∀t. (walk t responses result ⇒ walk (Tau t) responses result)) ∧ *)
+(* [~Vis:] (∀k e r. walk (k r) responses result *)
+(*            ⇒ walk (Vis e k) (r::responses) ((e,r)::result)) ∧ *)
+(* [~Ret:] (∀r. walk (Ret r) [] []) *)
+(* End *)
+
+Inductive next:
+  (P (Ret r) ⇒ next P (Ret r)) ∧
+  (P (Tau t) ⇒ next P t) ∧
+  ((∀a. P (k a)) ⇒ next P (Vis e k))
+End
+
+(* RTC of above *)
+Inductive future:
+  (P t ⇒ future P t) ∧
+  (future P t ⇒ future P (Tau t)) ∧
+  ((∀a. future P (k a)) ⇒ future P (Vis e k))
+End
+
+Definition the_ffi_def:
+  the_ffi t res f =
+  (∃q. t = (case res of
+              FFI_return new_ffi new_bytes => f new_ffi new_bytes
+            | FFI_final outcome => q outcome))
+End
+
+Theorem pull_ffi_case:
+  (to_ffi
+   (iter (mrec_cb h_prog)
+         (f (case res of
+               FFI_return new_ffi new_bytes => a new_ffi new_bytes
+             | FFI_final outcome => b outcome))))
+  =
+  (case res of
+     FFI_final outcome =>
+       to_ffi (iter (mrec_cb h_prog) (f (b outcome)))
+   | FFI_return new_ffi new_bytes =>
+       to_ffi (iter (mrec_cb h_prog) (f (a new_ffi new_bytes))))
 Proof
+  rw[FUN_EQ_THM] >>
+  Cases_on ‘res’ >> rw[]
+QED
+
+Theorem itree_wbisim_drop_tau:
+  ∀t. t ≈ t' ⇒ Tau t ≈ t
+Proof
+  metis_tac[itree_wbisim_tau_eq, itree_wbisim_trans]
+QED
+
+Theorem ffi_sem_thm:
+  future (λt. (∃k k'. (t = Vis (FFI_call "f3" [] []) k) ∧
+                      k (FFI_return ARB ARB) ≈ (Vis (FFI_call "f4" [] []) k')) ∨
+              (∃outcome. t = Ret (SOME (FinalFFI outcome))))
+  (ffi_sem s)
+Proof
+  qmatch_goalsub_abbrev_tac ‘future P (ffi_sem _)’ >>
   rw[ffi_sem_def, itree_semantics_def, itree_evaluate_alt] >>
+  (* Seq rw[seq_thm] *)
+  rw[itree_mrec_alt, h_prog_def, h_prog_rule_seq_def] >>
+  rw[Once itree_iter_thm, Once itree_bind_thm] >>
+  (* extcall *)
+  rw[itree_mrec_alt, h_prog_def, h_prog_rule_ext_call_def] >>
+  rw[eval_def, FLOOKUP_UPDATE] >>
+  rw[read_bytearray_def] >>
+  (* massaging *)
+  rw[Once future_cases] >> disj2_tac >>
+  rw[Once future_cases] >> disj2_tac >>
+  rw[Once future_cases] >> disj2_tac >>
+  rw[pull_ffi_case] >>
+  reverse (Cases_on ‘a’) >-
+   (fs[Once future_cases] >>
+    metis_tac[]) >>
+  rw[Once future_cases] >> disj2_tac >>
   (* Seq *)
   rw[itree_mrec_alt, h_prog_def, h_prog_rule_seq_def] >>
   rw[Once itree_iter_thm, Once itree_bind_thm] >>
@@ -360,13 +312,210 @@ Proof
   rw[itree_mrec_alt, h_prog_def, h_prog_rule_ext_call_def] >>
   rw[eval_def, FLOOKUP_UPDATE] >>
   rw[read_bytearray_def] >>
-  (* next, stuck *)
+  (* *)
+  rw[Once future_cases] >> disj2_tac >>
+  rw[Once future_cases] >> disj2_tac >>
+  rw[Once future_cases] >> disj2_tac >>
+  rw[pull_ffi_case] >>
+  reverse (Cases_on ‘a’) >-
+   (fs[Once future_cases] >>
+    metis_tac[]) >>
+  rw[Once future_cases] >> disj2_tac >>
+  (* extcall *)
+  rw[itree_mrec_alt, h_prog_def, h_prog_rule_ext_call_def] >>
+  rw[eval_def, FLOOKUP_UPDATE] >>
+  rw[read_bytearray_def] >>
+  (* seq *)
+  rw[itree_mrec_alt, h_prog_def, h_prog_rule_seq_def] >>
+  rw[Once itree_iter_thm, Once itree_bind_thm] >>
+  (* extcall *)
+  rw[itree_mrec_alt, h_prog_def, h_prog_rule_ext_call_def] >>
+  rw[eval_def, FLOOKUP_UPDATE] >>
+  rw[read_bytearray_def] >>
+  rw[Once future_cases] >> disj2_tac >>
+  rw[Once future_cases] >> disj1_tac >>
+  qunabbrev_tac ‘P’ >>
+  rw[] >>
+  (* extcall *)
+  rw[itree_mrec_alt, h_prog_def, h_prog_rule_ext_call_def] >>
+  rw[eval_def, FLOOKUP_UPDATE] >>
+  rw[read_bytearray_def] >>
+  metis_tac[itree_wbisim_drop_tau, itree_wbisim_trans, itree_wbisim_refl]
+QED
+
+(*/ loops work!
+   manual loop unrolling isn't too bad with equational rewrites
+ *)
+
+(* val loop_ast = rhs $ concl $ parse_pancake ‘ *)
+(* fun fn() { *)
+(*   var x = 1; *)
+(*   x = 0; *)
+(*   while (x < 1) { *)
+(*     x = x + 1; *)
+(*   } *)
+(* }’; *)
+
+(* Definition loop_sem_def: *)
+(*   loop_sem (s:('a,'ffi) panSem$state) = *)
+(*   itree_evaluate (SND $ SND $ HD $ THE ^loop_ast) s *)
+(* End *)
+
+(* Definition h_prog_whilebody_cb_def[simp]: *)
+(*     h_prog_whilebody_cb p (SOME Break) s' = Ret (INR (NONE,s')) *)
+(*   ∧ h_prog_whilebody_cb p (SOME Continue) s' = Ret (INL (p,s')) *)
+(*   ∧ h_prog_whilebody_cb p NONE s' = Ret (INL (p,s')) *)
+(*   (* nice! this syntax is valid *) *)
+(*   ∧ h_prog_whilebody_cb p res s' = Ret (INR (res,s')) *)
+(* End *)
+
+(* Definition h_prog_while_cb_def[simp]: *)
+(*     h_prog_while_cb (p,s) NONE = Ret (INR (SOME Error,s)) *)
+(*   ∧ h_prog_while_cb (p,s) (SOME (ValWord w)) *)
+(*     = (if (w ≠ 0w) *)
+(*        then Vis (INL (p,s)) *)
+(*                 (λ(res,s'). h_prog_whilebody_cb p res s') *)
+(*        else Ret (INR (NONE,s))) *)
+(*   ∧ h_prog_while_cb (p,s) (SOME (ValLabel _)) = Ret (INR (SOME Error,s)) *)
+(*   ∧ h_prog_while_cb (p,s) (SOME (Struct _)) = Ret (INR (SOME Error,s)) *)
+(* End *)
+
+(* (* PR submitted *) *)
+(* Theorem h_prog_rule_while_alt: *)
+(*   h_prog_rule_while g p s = *)
+(*   iter (λ(p',s'). (h_prog_while_cb (p',s') (eval s' g))) (p,s) *)
+(* Proof *)
+(*   rw[h_prog_rule_while_def] >> *)
+(*   AP_THM_TAC >> *)
+(*   AP_TERM_TAC >> *)
+(*   rw[FUN_EQ_THM] >> *)
+(*   rw[DefnBase.one_line_ify NONE h_prog_while_cb_def] >> *)
+(*   rw[DefnBase.one_line_ify NONE h_prog_whilebody_cb_def] >> *)
+(*   rpt (PURE_TOP_CASE_TAC >> gvs[] >> rw[FUN_EQ_THM]) *)
+(* QED *)
+
+(* Theorem cheat1: *)
+(*   0w < 1w (* supposed to be :4 word but weever *) *)
+(* Proof *)
+(*   cheat *)
+(* QED *)
+
+(* Theorem loop_thm: *)
+(*   loop_sem s =  Tau (Tau (Tau (Tau (Tau (Ret NONE))))) *)
+(* Proof *)
+(*   rw[loop_sem_def, itree_semantics_def, itree_evaluate_alt] >> *)
+(*   rw[itree_mrec_alt, h_prog_def, h_prog_rule_dec_alt] >> *)
+(*   rw[eval_def] >> *)
+(*   rw[Once itree_iter_thm, itree_bind_thm] >> *)
+(*   (* seq *) *)
+(*   rw[h_prog_def, h_prog_rule_seq_def] >> *)
+(*   rw[itree_bind_thm] >> *)
+(*   rw[Once itree_iter_thm] >> *)
+(*   rw[Once itree_bind_thm] >> *)
+(*   (* assign *) *)
+(*   rw[Once h_prog_def, h_prog_rule_assign_def] >> *)
+(*   rw[FLOOKUP_UPDATE, word_op_def, is_valid_value_def, shape_of_def, *)
+(*      Once eval_def, cheat1] >> *)
+(*   rw[itree_bind_thm] >> *)
+(*   rw[Once itree_iter_thm, Once itree_bind_thm] >> *)
+(*   (* while *) *)
+(*   rw[Once h_prog_def, h_prog_rule_while_alt] >> *)
+(*   rw[Once itree_iter_thm] >> rw[Once itree_iter_thm] >> *)
+(*   rw[Once eval_def] >> rw[Once eval_def] >> *)
+(*   rw[FLOOKUP_UPDATE] >> *)
+(*   rw[Once eval_def, word_cmp_def, cheat1] >> *)
+(*   rw[itree_bind_thm] >> *)
+(*   (* assignment *) *)
+(*   rw[Once h_prog_def, h_prog_rule_assign_def] >> *)
+(*   rw[Once eval_def] >> rw[Once eval_def] >> *)
+(*   rw[FLOOKUP_UPDATE, word_op_def, is_valid_value_def, shape_of_def, *)
+(*      Once eval_def, cheat1] >> *)
+(*   rw[Once itree_iter_thm, itree_bind_thm] >> *)
+(*   (* second while *) *)
+(*   (* rw[GSYM h_prog_rule_while_alt, GSYM h_prog_def] *) *)
+(*   rw[Once itree_iter_thm] >> rw[Once itree_iter_thm] >> *)
+(*   rw[eval_def, FLOOKUP_UPDATE, word_cmp_def] >> *)
+(*   rw[revert_binding_def] >> *)
+(*   rw[Once itree_iter_thm, itree_bind_thm] >> *)
+(*   (* massage *) *)
+(*   rw[massage_thm] *)
+(* QED *)
+
+(*/ interp nonsense
+   weird
+ *)
+
+Definition interp_cb_def[simp]:
+  interp_cb rh (Ret r) = Ret (INR r) ∧
+  interp_cb rh (Tau t) = Ret (INL t) ∧
+  interp_cb rh (Vis e k) = bind (rh e) (λa. Ret (INL (k a)))
+End
+
+(* (E -> itree E' R) -> itree E R -> itree E' R *)
+Definition itree_interp_def:
+  itree_interp rh it = itree_iter (interp_cb rh) it
+End
+
+Theorem interp_cb_ret_inv:
+  interp_cb rh t = Ret (INR r) ⇒ t = (Ret r)
+Proof
+  rw[DefnBase.one_line_ify NONE interp_cb_def] >>
+  Cases_on ‘t’ >> fs[] >>
+  Cases_on ‘rh a’ >> fs[]
+QED
+
+Theorem itree_interp_ret:
+  itree_interp rh (Ret r) = Ret r
+Proof
+  rw[itree_interp_def] >>
+  rw[Once itree_iter_thm]
+QED
+
+Theorem itree_interp_trigger:
+  itree_interp rh (Vis e Ret) ≈ rh e
+Proof
+  rw[itree_interp_def] >>
   rw[Once itree_iter_thm] >>
-  (* massaging *)
-  rw[to_ffi_def] >>
-  rw[Once itree_unfold] >>
-  rw[massage_def] >>
-  rw[Once itree_unfold] >>
-  rw[massage_def] >>
-  rw[combinTheory.o_DEF] >>
+  rw[itree_bind_assoc] >>
+  rw[Once itree_iter_thm] >>
+  irule itree_wbisim_coind >>
+  qexists_tac ‘λa b. ∃t. a = bind t (λa. Tau (Ret a)) ∧ b = t’ >>
+  rw[] >>
+  Cases_on ‘a1’ >> rw[]
+QED
+
+Theorem itree_interp_bind:
+  itree_interp rh (bind t k) = bind (itree_interp rh t) (λr. itree_interp rh (k r))
+Proof
+  rw[itree_interp_def] >>
+  rw[Once itree_strong_bisimulation] >>
+  qexists_tac ‘λa b. ∃ps. a = iter (interp_cb rh) (bind ps k) ∧
+                          b = bind (iter (interp_cb rh) ps)
+                                   (λx. iter (interp_cb rh) (k x))’ >>
+  rw[] >-
+   (metis_tac[])
+   (cheat
+   )
+QED
+
+(* they are only weakly bisimilar *)
+Theorem itree_mrec_interp:
+  iter (mrec_cb rh) t ≈
+  itree_interp (λe. case e of
+                      (INL a) => (itree_mrec rh a)
+                    | (INR e) => Vis e Ret)
+  t
+Proof
+  rw[Once itree_mrec_alt, itree_interp_def] >>
+  rw[Once itree_iter_thm] >>
+  CONV_TAC $ RHS_CONV $ ONCE_REWRITE_CONV[itree_iter_thm] >>
+  Cases_on ‘e’ >> rw[] >-
+   (rw[itree_bind_assoc] >>
+    rw[itree_mrec_bind] >>
+    rw[GSYM itree_mrec_alt] >>
+    cheat
+   ) >-
+   (rw[FUN_EQ_THM] >>
+    rw[]
+   )
 QED
